Start porting to vListInsert, laptop dying

timing/examples/FreeRTOS/list/vListInsert.v
@@ -38,68 +38,133 @@ Global Ltac Zify.zify_pre_hook ::= idtac.
 Definition portMAX_DELAY := 2^32 - 1.
 
 Definition time_of_vListInsert (mem : memory)
-    (pxNewListItem : addr) (maximal_index : N) (t : trace) :=
+    (pxNewListItem : addr) (le_index : N) (t : trace) :=
   cycle_count_of_trace t =
     tlw + taddi + taddi +
     (if mem Ⓓ[pxNewListItem] =? portMAX_DELAY then (
       tfbne + tlw
     ) else (
-      ttbne + (maximal_index - 1) * (
+      ttbne + le_index * (
         taddi + tlw + tlw + ttbgeu
       ) + taddi + tlw + tlw + tfbgeu + tjal
     )) + (
       tlw + 4 * tsw + tlw + tsw + taddi + tsw + tjalr
     ).
 
-Definition exists_maximal (mem : memory) (pxList pxNewListItem maximal : addr)
-    (max_val new_val : N) (max_dist : nat):=
-  node_distance mem pxList maximal max_dist /\
-  list_node_value mem maximal = Some max_val /\
-  max_val <= new_val /\
-  LLForall (fun m a => 
-    match list_node_value m a with
-    | None => True
-    | Some val => val <= max_val
-    end
-  ) mem pxList.
+Definition insertion_index mem l le_node le_dist le_val new_val len :=
+    exists gt_node gt_val,
+    node_distance mem l le_node le_dist /\
+    list_node_value mem le_node = Some le_val /\
+    list_node_next mem le_node = Some gt_node /\
+    list_node_value mem gt_node = Some gt_val /\
+    gt_node <> NULL /\
+    le_val <= new_val < gt_val /\
+    gt_val <= portMAX_DELAY /\
+    (le_dist < len)%nat /\
+    (* all nodes below le_dist satisfy n.val <= new_val *)
+    forall n d v,
+        node_distance mem l n d ->
+        list_node_value mem n = Some v ->
+        ((d <= le_dist)%nat <-> v <= new_val).
 
-Definition vListInsert_timing_invs (base_mem : memory) (len : nat) (max_val new_val : N)
-    (pxList pxNewListItem maximal : addr) (dist_to_maximal : nat) (t:trace) : option Prop :=
+Definition vListInsert_timing_invs (base_mem : memory)
+    (pxList pxNewListItem le_node sentry : addr) 
+    (new_val le_val : N)
+    (le_dist len : nat) (t:trace) : option Prop :=
 match t with (Addr a, s) :: t' => match a with
 | 0x800023f0 => Some (
-    exists_maximal (s V_MEM32) pxList pxNewListItem maximal
-      max_val new_val dist_to_maximal /\
-    s R_A0 = pxList /\ s R_A1 = pxNewListItem /\
-    s V_MEM32 = base_mem /\
-    pxList <> NULL /\
-    node_distance (s V_MEM32) pxList NULL len /\
+    insertion_index base_mem pxList le_node le_dist le_val new_val len /\
+    node_distance (s V_MEM32) pxList sentry (len - 1) /\
+    list_node_value (s V_MEM32) sentry = Some portMAX_DELAY /\
+    s R_A0 = pxList /\ s R_A1 = pxNewListItem /\ s V_MEM32 = base_mem /\
+    s V_MEM32 Ⓓ[pxNewListItem] = new_val /\
+    pxList <> NULL /\ len <> 0%nat /\
+    node_distance base_mem pxList NULL len /\
     cycle_count_of_trace t' = 0
   )
 | 0x8000242c => Some (exists ctr,
-    exists_maximal (s V_MEM32) pxList pxNewListItem maximal
-      max_val new_val dist_to_maximal /\
-    pxList <> NULL /\
-    s V_MEM32 = base_mem /\
+    insertion_index base_mem pxList le_node le_dist le_val new_val len /\
+    node_distance (s V_MEM32) pxList sentry (len - 1) /\
+    list_node_value (s V_MEM32) sentry = Some portMAX_DELAY /\
     (base_mem Ⓓ[pxNewListItem] =? portMAX_DELAY) = false /\
-    node_distance (s V_MEM32) pxList NULL len /\
-    node_distance (s V_MEM32) pxList ((s V_MEM32) Ⓓ[s R_A4]) ctr /\
+    s R_A0 <> NULL /\
+    pxList <> NULL /\ s V_MEM32 = base_mem /\
+    s R_A1 = pxNewListItem /\ s R_A3 = new_val /\
+    len <> 0%nat /\
+    (ctr <= le_dist)%nat /\
+    node_distance base_mem pxList NULL len /\
+    node_distance base_mem pxList (s R_A0) ctr /\
     cycle_count_of_trace t' =
       tlw + taddi + taddi +
-      ttbne + (N.of_nat ctr - 1) * (
+      ttbne + (N.of_nat ctr) * (
         taddi + tlw + tlw + ttbgeu
       )
   )
 | 0x80002428 => Some (time_of_vListInsert base_mem
-                    pxNewListItem (N.of_nat dist_to_maximal) t)
+                    pxNewListItem (N.of_nat le_dist) t)
 | _ => None end | _ => None end.
 
 Lemma le_cases : forall n m,
     (n <= m -> n < m \/ n = m)%nat.
 Proof. lia. Qed.
 
+Lemma not_at_end_next : forall mem head len a dist,
+    node_distance mem head NULL len ->
+    node_distance mem head a dist ->
+    (dist < len)%nat ->
+    exists val, list_node_next mem a = Some val.
+Proof.
+    intros. unfold list_node_next. destruct a.
+    - pose proof (node_distance_uniq _ _ _ _ _ H H0).
+        subst. lia.
+    - eexists. reflexivity.
+Qed.
+
+Lemma not_at_end_next' : forall mem head len a1 dist1 a2 dist2,
+    node_distance mem head NULL len ->
+    node_distance mem head a1 dist1 ->
+    node_distance mem head a2 dist2 ->
+    (dist2 < dist1 <= len)%nat ->
+    exists val2, list_node_next mem a2 = Some val2.
+Proof.
+    intros. unfold list_node_next. destruct a2.
+    - pose proof (node_distance_uniq _ _ _ _ _ H H1).
+        subst. lia.
+    - eexists. reflexivity.
+Qed.
+
+Lemma head_nonnull_impl_len_nonzero : forall mem head len,
+    node_distance mem head NULL len ->
+    head <> NULL ->
+    len <> 0%nat.
+Proof.
+    intros. destruct len.
+    - inversion H. contradiction.
+    - discriminate.
+Qed.
+
+Lemma at_end_lens : forall mem head len a dst,
+    head <> NULL ->
+    node_distance mem head NULL len ->
+    node_distance mem head a dst ->
+    list_node_next mem a = Some NULL ->
+    S dst = len.
+Proof.
+    intros. destruct a.
+    - inversion H2.
+    - pose proof (node_distance_len_nonzero _ _ _ H0).
+        change NULL with LL.NULL in *.
+        apply N.eqb_neq in H. rewrite H in H3.
+        specialize (H3 ltac:(reflexivity)).
+        pose proof distance_last_node.
+        unfold LL.NULL in H4.
+        specialize (H4 mem head (N.pos p) dst ltac:(lia) H1 H2).
+        pose proof (node_distance_uniq _ _ _ _ _ H0 H4).
+        now symmetry.
+Qed.
+
 Theorem vListInsert_timing:
-  forall s t s' x' base_mem len pxList pxNewListItem maximal max_val
-            dist_to_maximal new_val
+  forall s t s' x' base_mem len pxList pxNewListItem le_node le_dist le_val sentry new_val
          (* boilerplate *)
          (ENTRY: startof t (x',s') = (Addr entry_addr, s))
          (MDL: models rvtypctx s)
@@ -107,17 +172,20 @@ Theorem vListInsert_timing:
          (MEM: s V_MEM32 = base_mem)
          (A0: s R_A0 = pxList)
          (A1: s R_A1 = pxNewListItem)
-         (* pxList is non-null (guaranteed by vListInitialise) *)
-         (PXL_NN: pxList <> NULL)
+         (* contents of pxNewListItem *)
+         (VAL: s V_MEM32 Ⓓ[pxNewListItem] = new_val)
          (* list length is finite *)
          (LEN: node_distance (s V_MEM32) pxList NULL len)
-         (NLI_VAL: list_node_value base_mem pxNewListItem = Some new_val)
-         (* there exists a maximal node in the list with a value
-            less than or equal to that of pxNewListItem *)
-         (MAX: exists_maximal base_mem pxList pxNewListItem maximal max_val new_val dist_to_maximal),
+         (* pxList is non-null *)
+         (L_NN: pxList <> NULL)
+         (* there is a sentry node *)
+         (SENTRY: node_distance (s V_MEM32) pxList sentry (len - 1))
+         (SENTRY_VAL: list_node_value (s V_MEM32) sentry = Some portMAX_DELAY)
+         (* there is an index to insert at *)
+         (IDX: insertion_index base_mem pxList le_node le_dist le_val new_val len),
   satisfies_all
     lifted_prog
-    (vListInsert_timing_invs base_mem len max_val new_val pxList pxNewListItem maximal dist_to_maximal)
+    (vListInsert_timing_invs base_mem pxList pxNewListItem le_node sentry new_val le_val le_dist len)
     exits
   ((x',s')::t).
 Proof using.
@@ -125,9 +193,9 @@ Proof using.
     apply prove_invs.
 
     Local Ltac step := tstep r5_step.
-    simpl. rewrite ENTRY. unfold entry_addr. step.
-    rewrite MEM.
+    simpl. rewrite ENTRY. unfold entry_addr. repeat step.
     split. assumption. repeat split; auto.
+    eapply head_nonnull_impl_len_nonzero; eassumption.
     now rewrite <- MEM.
 
     intros.
@@ -138,45 +206,78 @@ Proof using.
 
     destruct_inv 32 PRE.
 
-    - destruct PRE as (EMax & A0 & A1 & MEM & PXL_NN & Len & Cycles).
-      repeat step.
-      -- (* 0x8000242c invariant *)
-        exists 1%nat. rewrite MEM in *. split. assumption.
-        repeat split; auto.
-        now apply Bool.negb_true_iff in BC. 
-        apply node_distance_next_S_len with (dst := pxList).
-          unfold list_node_next. destruct pxList.
-            contradiction.
-            reflexivity.
-          eapply distance_null_imp_well_formed; eassumption.
-          apply Dst0.
-          hammer.
-      -- (* 0x80002428 postcondition *)
-        unfold portMAX_DELAY.
-        hammer.
-    - destruct PRE as (ctr & EMax & PXL_NN & MEM & NLI_VALID & Len & DstCurr & 
-          Cycles).
-      repeat step.
-      -- (* 0x80002428 postcondition *)
-        rewrite NLI_VALID.
-        hammer. replace ctr with dist_to_maximal.
-        lia.
-        destruct EMax, H0, H1.
-        enough (s' V_MEM32 Ⓓ[s' R_A4] = maximal).
-          rewrite H3 in *.
-          eapply node_distance_uniq; eassumption.
-        (* If we can show that we have reached the maximal 
-           list item, this is proven
-        *)
-        admit.
-      -- exists (S ctr). rewrite MEM in *.
-         split. assumption. repeat split; auto.
-         eapply node_distance_next_S_len; eauto.
-         unfold list_node_next.
-         admit.
-         eapply distance_null_imp_well_formed; eassumption.
-         replace (N.of_nat (S ctr) - 1) with (N.of_nat ctr) by lia.
-         hammer. replace (N.of_nat ctr) with (1 + N.of_nat ctr - 1) at 2 by lia.
-         rewrite <- N.add_sub_assoc. lia.
-         admit.
+    - destruct PRE as (IDX & SENTRY & SENTRY_VAL & A0 & A1 & MEM & NewVal & NonNull & L_NN & Len_Nz & Cycles).
+        do 4 step.
+        -- exists 0%nat. split. assumption.
+            repeat split; auto; try now rewrite <- MEM.
+            unfold portMAX_DELAY. lia. lia.
+            apply Dst0.
+            hammer.
+        -- repeat step. unfold portMAX_DELAY. hammer.
+    - destruct PRE as (ctr & IDX & SENTRY & SENTRY_VAL & ValueValid & A0 & L_NN & MEM & A1 & A3 & Len_Nz & CtrMax &
+                        Len & CtrDist & Cycles).
+        repeat step.
+        -- hammer. replace ctr with le_dist.
+            hammer.
+            destruct (le_cases ctr le_dist CtrMax); try lia.
+            clear - H CtrDist IDX Len Len_Nz BC A0.
+            destruct IDX as (gt_node & gt_val & LeDist & LeVal & LeNextGt & GtVal & _ & Vals & _ & Lens & Sorted).
+            exfalso.
+            pose proof (not_at_end_next _ _ _ _ _ Len CtrDist ltac:(lia)).
+            destruct H0 as (a0nxt & a0eq).
+            specialize (Sorted a0nxt (S ctr) (base_mem Ⓓ[base_mem Ⓓ[4 + s' R_A0]])).
+            pose proof (node_distance_next_S_len _ _ _ _ _ a0eq (distance_null_imp_well_formed _ _ _ Len) CtrDist).
+            specialize (Sorted H0).
+            enough (list_node_value base_mem a0nxt = Some (base_mem Ⓓ[base_mem Ⓓ[ 4 + s' R_A0 ]])).
+            destruct (s' R_A0).
+                contradiction.
+            specialize (Sorted H1).
+            apply N.ltb_lt in BC. lia.
+            pose proof (not_at_end_next _ _ _ _ _ Len H0 ltac:(lia)).
+            destruct H1 as (a0nxt2 & a0eq2).
+            destruct a0nxt eqn:E. inversion a0eq2.
+            unfold list_node_value. rewrite <- E in *; clear E.
+            replace a0nxt with (base_mem Ⓓ[ 4 + s' R_A0 ]). reflexivity.
+            destruct (s' R_A0). contradiction.
+                unfold list_node_next in a0eq.
+                change 4 with p.dw. remember (p.dw + N.pos p0).
+                injection a0eq. now intro.
+        -- exists (S ctr). split. assumption.
+            destruct IDX as (gt_node & gt_val & LeDist & LeVal & LeNextGt & GtVal & GtNN & Vals & MaxVal & Lens & Sorted).
+            repeat split; auto; try lia; try now rewrite <- MEM.
+            intro Contra.
+                replace sentry with (s' R_A0) in *.
+                rewrite MEM in *.
+                specialize (Sorted _ _ _ SENTRY SENTRY_VAL).
+                destruct (Nat.le_gt_cases (len - 1) le_dist). lia.
+                assert (S ctr < len)%nat by lia.
+                pose proof (at_end_lens _ _ _ _ _ L_NN Len CtrDist).
+                destruct H1; try lia.
+                destruct (s' R_A0). contradiction. change 4 with p.dw in Contra.
+                unfold list_node_next. f_equal. apply Contra.
+                pose proof (distance_last_node base_mem l (s' R_A0) ctr A0 CtrDist).
+                destruct (s' R_A0). contradiction. unfold list_node_next in H.
+                unfold p.w, p.e, p.pw, p.dw in H. rewrite Contra in H.
+                specialize (H ltac:(reflexivity)).
+                assert (S ctr = len) by eauto using node_distance_uniq.
+                subst len. simpl in SENTRY. rewrite Nat.sub_0_r in SENTRY.
+                eapply node_distance_uniq'; eauto. now rewrite <- MEM.
+            destruct (le_cases ctr le_dist CtrMax). lia.
+                subst ctr.
+                pose proof (node_distance_uniq' _ _ _ _ _ _ LeDist CtrDist eq_refl).
+                subst le_node.
+                apply N.ltb_ge in BC.
+                (* specialize (Sorted _ _ _ LeDist ltac:(lia) LeVal). *)
+                destruct (s' R_A0). contradiction.
+                replace gt_node with (base_mem Ⓓ[4 + N.pos p]) in *.
+                destruct (base_mem Ⓓ[ 4 + N.pos p ]). contradiction.
+                    inversion GtVal. subst gt_val. clear - Vals BC.
+                    replace (getmem p.w p.e p.dw base_mem (N.pos p0)) with (base_mem Ⓓ[N.pos p0]) in Vals by reflexivity.
+                    lia.
+                destruct (N.pos p). contradiction. now inversion LeNextGt.
+            eapply node_distance_next_S_len with (dst := s' R_A0).
+                destruct (s' R_A0). contradiction. reflexivity.
+            eapply distance_null_imp_well_formed. now eassumption.
+            assumption.
+            hammer.
 Admitted.
